IMPminus_TM/GOTO_WHILE/While_Prog_Gen.thy
@@ -1,0 +1,410 @@
+theory While_Prog_Gen
+  imports "IMPminus_TM-Def.GOTO" "IMP_Minus.Com" "IMP_Minus.Big_StepT"
+begin
+
+fun well_defined_instr :: "instr \<Rightarrow> bool" where
+  "well_defined_instr HALT = True" | 
+  "well_defined_instr (x ::= t) = (x \<noteq> ''pc''\<and> (case t of N c \<Rightarrow> True | V y \<Rightarrow> y \<noteq> ''pc''))" |
+  "well_defined_instr (x += t) = (x \<noteq> ''pc''\<and> (case t of N c \<Rightarrow> True | V y \<Rightarrow> y \<noteq> ''pc''))" |
+  "well_defined_instr (x -= t) = (x \<noteq> ''pc'' \<and> (case t of N c \<Rightarrow> True | V y \<Rightarrow> y \<noteq> ''pc''))" |
+  "well_defined_instr (x \<bind>1) = (x \<noteq> ''pc'')" |
+  "well_defined_instr (x %=2) = (x \<noteq> ''pc'')" |
+  "well_defined_instr (GOTO i) = True" |
+  "well_defined_instr (IF x\<noteq>0 THEN GOTO i) = (x \<noteq> ''pc'')"
+
+fun GOTO_instr_to_WHILE :: "instr \<Rightarrow> com" where
+  "GOTO_instr_to_WHILE HALT = ''pc'' ::= A (atomExp.N 0)" | 
+  "GOTO_instr_to_WHILE (x ::= t) = 
+    (case t of operi.N c \<Rightarrow> x ::= A (atomExp.N c) | operi.V y \<Rightarrow> x ::= A (atomExp.V y)) ;; 
+    ''pc'' ::= (atomExp.V ''pc'' \<oplus> atomExp.N 1)" | 
+  "GOTO_instr_to_WHILE (x += t) = 
+    (case t of operi.N c \<Rightarrow> x ::= (atomExp.V x \<oplus> atomExp.N c) | operi.V y \<Rightarrow> x ::= (atomExp.V x \<oplus> atomExp.V y)) ;; 
+    ''pc'' ::= (atomExp.V ''pc'' \<oplus> atomExp.N 1)" |
+  "GOTO_instr_to_WHILE (x -= t) = 
+    (case t of operi.N c \<Rightarrow> x ::= (atomExp.V x \<ominus> atomExp.N c) | operi.V y \<Rightarrow> x ::= (atomExp.V x \<ominus> atomExp.V y)) ;; 
+    ''pc'' ::= (atomExp.V ''pc'' \<oplus> atomExp.N 1)" | 
+  "GOTO_instr_to_WHILE (x \<bind>1) = 
+    x ::= (atomExp.V x \<then>) ;; 
+    ''pc'' ::= (atomExp.V ''pc'' \<oplus> atomExp.N 1)" | 
+  "GOTO_instr_to_WHILE (x %=2) = 
+    x ::= (atomExp.V x \<doteq>1) ;; 
+    ''pc'' ::= (atomExp.V ''pc'' \<oplus> atomExp.N 1)" | 
+  "GOTO_instr_to_WHILE (GOTO i) = ''pc'' ::= A (atomExp.N i)" | 
+  "GOTO_instr_to_WHILE (IF x\<noteq>0 THEN GOTO i) = IF x\<noteq>0 THEN ''pc'' ::= A (atomExp.N i) ELSE ''pc'' ::= (atomExp.V ''pc'' \<oplus> atomExp.N 1)"
+
+lemma pc_consist:
+  assumes "well_defined_instr instr"
+    and "(GOTO_instr_to_WHILE instr, s) \<Rightarrow>\<^bsup> k \<^esup> t"
+    and "iexec instr (pc, s') = (pc', t')" 
+    and "s ''pc'' = pc" and "\<forall>x \<noteq> ''pc''. s x = s' x"
+  shows "t ''pc'' = pc'"
+proof (cases instr)
+  case HALT
+  have "(''pc'' ::= A (atomExp.N 0), s) \<Rightarrow>\<^bsup> k \<^esup> t" using HALT assms(2) by auto
+  hence "s(''pc'' := aval (A (atomExp.N 0)) s) = t" by blast
+  hence aux1: "t ''pc'' = 0" by force
+
+  have "iexec HALT (pc, s') = (0, s')" by simp
+  hence aux2: "pc' = 0" using HALT assms(3) by force
+
+  show ?thesis using aux1 aux2 by simp
+next
+  case (ASSIGN x tmp)
+  then show ?thesis
+  proof (cases tmp)
+    case (N c)
+    let ?inter = "s(x := c)"
+    let ?final = "?inter(''pc'' := ?inter ''pc'' + 1)"
+    let ?w_com = "x ::= A (atomExp.N c) ;; ''pc'' ::= (atomExp.V ''pc'' \<oplus> atomExp.N 1)"
+    have aux1: "(x ::= A (atomExp.N c), s) \<Rightarrow>\<^bsup> 2 \<^esup> ?inter" by (simp add: AssignI')
+    have aux2: "(''pc'' ::= (atomExp.V ''pc'' \<oplus> atomExp.N 1), ?inter) \<Rightarrow>\<^bsup> 2 \<^esup> ?inter(''pc'' := ?inter ''pc'' + 1)" by (simp add: AssignI')
+    have "(?w_com, s) \<Rightarrow>\<^bsup> 4 \<^esup> ?inter(''pc'' := ?inter ''pc'' + 1)" using aux1 aux2 by (simp add: Seq)
+    hence "t = ?inter(''pc'' := ?inter ''pc'' + 1)" using ASSIGN N assms(2) by auto
+    hence aux3: "t ''pc'' = pc + 1" using ASSIGN assms(1) assms(4) by auto
+
+    have "iexec (x ::= tmp) (pc, s') = (pc + 1, s'(x := c))" by (simp add: N)
+    hence aux4: "pc' = pc + 1" using ASSIGN assms(3) by auto
+
+    show ?thesis using aux3 aux4 by blast
+  next
+    case (V y)
+    let ?inter = "s(x := s y)"
+    let ?final = "?inter(''pc'' := ?inter ''pc'' + 1)"
+    let ?w_com = "x ::= A (atomExp.V y) ;; ''pc'' ::= (atomExp.V ''pc'' \<oplus> atomExp.N 1)"
+    have aux1: "(x ::= A (atomExp.V y), s) \<Rightarrow>\<^bsup> 2 \<^esup> ?inter" by (simp add: AssignI')
+    have aux2: "(''pc'' ::= (atomExp.V ''pc'' \<oplus> atomExp.N 1), ?inter) \<Rightarrow>\<^bsup> 2 \<^esup> ?inter(''pc'' := ?inter ''pc'' + 1)" by (simp add: AssignI')
+    have "(?w_com, s) \<Rightarrow>\<^bsup> 4 \<^esup> ?inter(''pc'' := ?inter ''pc'' + 1)" using aux1 aux2 by (simp add: Seq)
+    hence "t = ?inter(''pc'' := ?inter ''pc'' + 1)" using ASSIGN V assms(2) by auto
+    hence aux3: "t ''pc'' = pc + 1" using ASSIGN assms(1) assms(4) by auto
+
+    have "iexec (x ::= tmp) (pc, s') = (pc + 1, s'(x := s' y))" by (simp add: V)
+    hence aux4: "pc' = pc + 1" using ASSIGN assms(3) by auto
+
+    show ?thesis using aux3 aux4 by blast
+  qed
+next
+  case (ADD x tmp)
+  then show ?thesis
+  proof (cases tmp)
+    case (N c)
+    let ?inter = "s(x := s x + c)"
+    let ?final = "?inter(''pc'' := ?inter ''pc'' + 1)"
+    let ?w_com = "x ::= (atomExp.V x \<oplus> atomExp.N c) ;; ''pc'' ::= (atomExp.V ''pc'' \<oplus> atomExp.N 1)"
+    have aux1: "(x ::= (atomExp.V x \<oplus> atomExp.N c), s) \<Rightarrow>\<^bsup> 2 \<^esup> ?inter" by (simp add: AssignI')
+    have aux2: "(''pc'' ::= (atomExp.V ''pc'' \<oplus> atomExp.N 1), ?inter) \<Rightarrow>\<^bsup> 2 \<^esup> ?inter(''pc'' := ?inter ''pc'' + 1)" by (simp add: AssignI')
+    have "(?w_com, s) \<Rightarrow>\<^bsup> 4 \<^esup> ?inter(''pc'' := ?inter ''pc'' + 1)" using aux1 aux2 by (simp add: Seq)
+    hence "t = ?inter(''pc'' := ?inter ''pc'' + 1)" using ADD N assms(2) by auto
+    hence aux3: "t ''pc'' = pc + 1" using ADD assms(1) assms(4) by auto
+
+    have "iexec (x += tmp) (pc, s') = (pc + 1, s'(x :=  s' x + c))" by (simp add: N)
+    hence aux4: "pc' = pc + 1" using ADD assms(3) by auto
+
+    show ?thesis using aux3 aux4 by blast
+  next
+    case (V y)
+    let ?inter = "s(x := s x + s y)"
+    let ?final = "?inter(''pc'' := ?inter ''pc'' + 1)"
+    let ?w_com = "x ::= (atomExp.V x \<oplus> atomExp.V y) ;; ''pc'' ::= (atomExp.V ''pc'' \<oplus> atomExp.N 1)"
+    have aux1: "(x ::= (atomExp.V x \<oplus> atomExp.V y), s) \<Rightarrow>\<^bsup> 2 \<^esup> ?inter" by (simp add: AssignI')
+    have aux2: "(''pc'' ::= (atomExp.V ''pc'' \<oplus> atomExp.N 1), ?inter) \<Rightarrow>\<^bsup> 2 \<^esup> ?inter(''pc'' := ?inter ''pc'' + 1)" by (simp add: AssignI')
+    have "(?w_com, s) \<Rightarrow>\<^bsup> 4 \<^esup> ?inter(''pc'' := ?inter ''pc'' + 1)" using aux1 aux2 by (simp add: Seq)
+    hence "t = ?inter(''pc'' := ?inter ''pc'' + 1)" using ADD V assms(2) by auto
+    hence aux3: "t ''pc'' = pc + 1" using ADD assms(1) assms(4) by auto
+
+    have "iexec (x += tmp) (pc, s') = (pc + 1, s'(x :=  s' x + s' y))" by (simp add: V)
+    hence aux4: "pc' = pc + 1" using ADD assms(3) by auto
+
+    show ?thesis using aux3 aux4 by blast
+  qed
+next
+  case (SUB x tmp)
+  then show ?thesis
+  proof (cases tmp)
+    case (N c)
+    let ?inter = "s(x := s x - c)"
+    let ?final = "?inter(''pc'' := ?inter ''pc'' + 1)"
+    let ?w_com = "x ::= (atomExp.V x \<ominus> atomExp.N c) ;; ''pc'' ::= (atomExp.V ''pc'' \<oplus> atomExp.N 1)"
+    have aux1: "(x ::= (atomExp.V x \<ominus> atomExp.N c), s) \<Rightarrow>\<^bsup> 2 \<^esup> ?inter" by (simp add: AssignI')
+    have aux2: "(''pc'' ::= (atomExp.V ''pc'' \<oplus> atomExp.N 1), ?inter) \<Rightarrow>\<^bsup> 2 \<^esup> ?inter(''pc'' := ?inter ''pc'' + 1)" by (simp add: AssignI')
+    have "(?w_com, s) \<Rightarrow>\<^bsup> 4 \<^esup> ?inter(''pc'' := ?inter ''pc'' + 1)" using aux1 aux2 by (simp add: Seq)
+    hence "t = ?inter(''pc'' := ?inter ''pc'' + 1)" using SUB N assms(2) by auto
+    hence aux3: "t ''pc'' = pc + 1" using SUB assms(1) assms(4) by auto
+
+    have "iexec (x -= tmp) (pc, s') = (pc + 1, s'(x :=  s' x - c))" by (simp add: N)
+    hence aux4: "pc' = pc + 1" using SUB assms(3) by auto
+
+    show ?thesis using aux3 aux4 by blast
+  next
+    case (V y)
+    let ?inter = "s(x := s x - s y)"
+    let ?final = "?inter(''pc'' := ?inter ''pc'' + 1)"
+    let ?w_com = "x ::= (atomExp.V x \<ominus> atomExp.V y) ;; ''pc'' ::= (atomExp.V ''pc'' \<oplus> atomExp.N 1)"
+    have aux1: "(x ::= (atomExp.V x \<ominus> atomExp.V y), s) \<Rightarrow>\<^bsup> 2 \<^esup> ?inter" by (simp add: AssignI')
+    have aux2: "(''pc'' ::= (atomExp.V ''pc'' \<oplus> atomExp.N 1), ?inter) \<Rightarrow>\<^bsup> 2 \<^esup> ?inter(''pc'' := ?inter ''pc'' + 1)" by (simp add: AssignI')
+    have "(?w_com, s) \<Rightarrow>\<^bsup> 4 \<^esup> ?inter(''pc'' := ?inter ''pc'' + 1)" using aux1 aux2 by (simp add: Seq)
+    hence "t = ?inter(''pc'' := ?inter ''pc'' + 1)" using SUB V assms(2) by auto
+    hence aux3: "t ''pc'' = pc + 1" using SUB assms(1) assms(4) by auto
+
+    have "iexec (x -= tmp) (pc, s') = (pc + 1, s'(x :=  s' x - s' y))" by (simp add: V)
+    hence aux4: "pc' = pc + 1" using SUB assms(3) by auto
+
+    show ?thesis using aux3 aux4 by blast
+  qed
+next
+  case (RSH x)
+  let ?inter = "s(x := s x div 2)"
+  let ?final = "?inter(''pc'' := ?inter ''pc'' + 1)"
+  let ?w_com = "x ::= (atomExp.V x \<then>) ;; ''pc'' ::= (atomExp.V ''pc'' \<oplus> atomExp.N 1)"
+  have aux1: "(x ::= (atomExp.V x \<then>), s) \<Rightarrow>\<^bsup> 2 \<^esup> ?inter" by (simp add: AssignI')
+  have aux2: "(''pc'' ::= (atomExp.V ''pc'' \<oplus> atomExp.N 1), ?inter) \<Rightarrow>\<^bsup> 2 \<^esup> ?inter(''pc'' := ?inter ''pc'' + 1)" by (simp add: AssignI')
+  have "(?w_com, s) \<Rightarrow>\<^bsup> 4 \<^esup> ?inter(''pc'' := ?inter ''pc'' + 1)" using aux1 aux2 by (simp add: Seq)
+  hence "t = ?inter(''pc'' := ?inter ''pc'' + 1)" using RSH assms(2) by auto
+  hence aux3: "t ''pc'' = pc + 1" using RSH assms(1) assms(4) by auto
+
+  have "iexec (x \<bind>1) (pc, s') = (pc + 1, s'(x :=  s' x div 2))" by simp
+  hence aux4: "pc' = pc + 1" using RSH assms(3) by auto
+  
+  show ?thesis using aux3 aux4 by blast
+next
+  case (MOD x)
+  let ?inter = "s(x := s x mod 2)"
+  let ?final = "?inter(''pc'' := ?inter ''pc'' + 1)"
+  let ?w_com = "x ::= (atomExp.V x \<doteq>1) ;; ''pc'' ::= (atomExp.V ''pc'' \<oplus> atomExp.N 1)"
+  have aux1: "(x ::= (atomExp.V x \<doteq>1), s) \<Rightarrow>\<^bsup> 2 \<^esup> ?inter" by (simp add: AssignI')
+  have aux2: "(''pc'' ::= (atomExp.V ''pc'' \<oplus> atomExp.N 1), ?inter) \<Rightarrow>\<^bsup> 2 \<^esup> ?inter(''pc'' := ?inter ''pc'' + 1)" by (simp add: AssignI')
+  have "(?w_com, s) \<Rightarrow>\<^bsup> 4 \<^esup> ?inter(''pc'' := ?inter ''pc'' + 1)" using aux1 aux2 by (simp add: Seq)
+  hence "t = ?inter(''pc'' := ?inter ''pc'' + 1)" using MOD assms(2) by auto
+  hence aux3: "t ''pc'' = pc + 1" using MOD assms(1) assms(4) by auto
+
+  have "iexec (x %=2) (pc, s') = (pc + 1, s'(x :=  s' x mod 2))" by simp
+  hence aux4: "pc' = pc + 1" using MOD assms(3) by auto
+  
+  show ?thesis using aux3 aux4 by blast
+next
+  case (JMP i)
+  have "(''pc'' ::= A (atomExp.N i), s) \<Rightarrow>\<^bsup> 2 \<^esup> s(''pc'' := i)" by (simp add: AssignI')
+  hence aux1: "t ''pc'' = i" using JMP assms(2) by auto
+
+  have "iexec (GOTO i) (pc, s') = (i, s')" by simp
+  hence aux2: "pc' = i" using JMP assms(3) by auto
+
+  show ?thesis using aux1 aux2 by blast
+next
+  case (CONDJMP x i)
+  let ?w_com = "IF x\<noteq>0 THEN ''pc'' ::= A (atomExp.N i) ELSE ''pc'' ::= (atomExp.V ''pc'' \<oplus> atomExp.N 1)"
+  consider (c1) "s x = 0" | (c2) "s x > 0" by auto
+  then show ?thesis
+  proof cases
+    case c1
+    have "(''pc'' ::= (atomExp.V ''pc'' \<oplus> atomExp.N 1), s) \<Rightarrow>\<^bsup> 2 \<^esup> s(''pc'' := s ''pc'' + 1)" by (simp add: AssignI')
+    hence "(?w_com, s) \<Rightarrow>\<^bsup> 3 \<^esup> s(''pc'' := s ''pc'' + 1)" by (simp add: big_step_t.IfFalse c1)
+    hence "t = s(''pc'' := s ''pc'' + 1)" using CONDJMP assms(2) by auto
+    hence aux1: "t ''pc'' = pc + 1" using CONDJMP assms(1) assms(4) by auto
+
+    have "iexec (IF x\<noteq>0 THEN GOTO i) (pc, s') = (pc + 1, s')" using c1 CONDJMP assms(1) assms(5) by auto
+    hence aux2: "pc' = pc + 1" using CONDJMP assms(3) by auto
+
+    show ?thesis using aux1 aux2 by blast
+  next
+    case c2
+    have "(''pc'' ::= A (atomExp.N i), s) \<Rightarrow>\<^bsup> 2 \<^esup> s(''pc'' := i)" by (simp add: AssignI')
+    hence "(?w_com, s) \<Rightarrow>\<^bsup> 3 \<^esup> s(''pc'' := i)" by (simp add: big_step_t.IfTrue c2)
+    hence aux1: "t ''pc'' = i" using CONDJMP assms(2) fun_upd_eqD by fastforce
+
+    have "iexec (IF x\<noteq>0 THEN GOTO i) (pc, s') = (i, s')" using CONDJMP assms(1) assms(5) c2 by auto
+    hence aux2: "pc' = i" using CONDJMP assms(3) by auto
+
+    show ?thesis using aux1 aux2 by blast
+  qed
+qed
+
+lemma aux_lemma1: "\<forall>x \<noteq> t. s x = s' x \<Longrightarrow> y \<noteq> t \<Longrightarrow> z \<noteq> t \<Longrightarrow> (s(x := s y)) z = (s'(x := s' y)) z" by simp
+
+lemma var_consist:
+  assumes "well_defined_instr instr"
+    and "(GOTO_instr_to_WHILE instr, s) \<Rightarrow>\<^bsup> k \<^esup> t"
+    and "iexec instr (pc, s') = (pc', t')" 
+    and "s ''pc'' = pc" and "\<forall>x \<noteq> ''pc''. s x = s' x"
+  shows "\<forall>z \<noteq> ''pc''. t z = t' z"
+proof (cases instr)
+  case HALT
+  have "(''pc'' ::= A (atomExp.N 0), s) \<Rightarrow>\<^bsup> k \<^esup> t" using HALT assms(2) by auto
+  hence "t = s(''pc'' := aval (A (atomExp.N 0)) s)" by blast
+  thus ?thesis using HALT assms(3) assms(5) by auto
+next
+  case (ASSIGN x tmp)
+  then show ?thesis
+  proof (cases tmp)
+    case (N c)
+    let ?inter = "s(x := c)"
+    let ?final = "?inter(''pc'' := ?inter ''pc'' + 1)"
+    let ?w_com = "x ::= A (atomExp.N c) ;; ''pc'' ::= (atomExp.V ''pc'' \<oplus> atomExp.N 1)"
+    have aux1: "(x ::= A (atomExp.N c), s) \<Rightarrow>\<^bsup> 2 \<^esup> ?inter" by (simp add: AssignI')
+    have aux2: "(''pc'' ::= (atomExp.V ''pc'' \<oplus> atomExp.N 1), ?inter) \<Rightarrow>\<^bsup> 2 \<^esup> ?inter(''pc'' := ?inter ''pc'' + 1)" by (simp add: AssignI')
+    have "(?w_com, s) \<Rightarrow>\<^bsup> 4 \<^esup> ?inter(''pc'' := ?inter ''pc'' + 1)" using aux1 aux2 by (simp add: Seq)
+    hence aux3: "t = ?inter(''pc'' := ?inter ''pc'' + 1)" using ASSIGN N assms(2) by auto
+
+    have "iexec (x ::= tmp) (pc, s') = (pc + 1, s'(x := c))" by (simp add: N)
+    hence aux4: "t' = s'(x := c)" using ASSIGN assms(3) by auto
+
+    show ?thesis using aux3 aux4 by (simp add: assms(5))
+  next
+    case (V y)
+    let ?inter = "s(x := s y)"
+    let ?final = "?inter(''pc'' := ?inter ''pc'' + 1)"
+    let ?w_com = "x ::= A (atomExp.V y) ;; ''pc'' ::= (atomExp.V ''pc'' \<oplus> atomExp.N 1)"
+    have aux1: "(x ::= A (atomExp.V y), s) \<Rightarrow>\<^bsup> 2 \<^esup> ?inter" by (simp add: AssignI')
+    have aux2: "(''pc'' ::= (atomExp.V ''pc'' \<oplus> atomExp.N 1), ?inter) \<Rightarrow>\<^bsup> 2 \<^esup> ?inter(''pc'' := ?inter ''pc'' + 1)" by (simp add: AssignI')
+    have "(?w_com, s) \<Rightarrow>\<^bsup> 4 \<^esup> ?inter(''pc'' := ?inter ''pc'' + 1)" using aux1 aux2 by (simp add: Seq)
+    hence aux3: "t = ?inter(''pc'' := ?inter ''pc'' + 1)" using ASSIGN V assms(2) by auto
+
+    have "iexec (x ::= tmp) (pc, s') = (pc + 1, s'(x := s' y))" by (simp add: V)
+    hence aux4: "t' = s'(x := s' y)" using ASSIGN assms(3) by auto
+
+    let ?inter' = "s'(x := s' y)"
+    have "\<forall>z \<noteq> ''pc''. ?inter z = ?inter' z" using ASSIGN V assms(1) assms(5) by auto
+    thus ?thesis using aux3 aux4 by simp
+  qed
+next
+  case (ADD x tmp)
+  then show ?thesis
+  proof (cases tmp)
+    case (N c)
+    let ?inter = "s(x := s x + c)"
+    let ?final = "?inter(''pc'' := ?inter ''pc'' + 1)"
+    let ?w_com = "x ::= (atomExp.V x \<oplus> atomExp.N c) ;; ''pc'' ::= (atomExp.V ''pc'' \<oplus> atomExp.N 1)"
+    have aux1: "(x ::= (atomExp.V x \<oplus> atomExp.N c), s) \<Rightarrow>\<^bsup> 2 \<^esup> ?inter" by (simp add: AssignI')
+    have aux2: "(''pc'' ::= (atomExp.V ''pc'' \<oplus> atomExp.N 1), ?inter) \<Rightarrow>\<^bsup> 2 \<^esup> ?inter(''pc'' := ?inter ''pc'' + 1)" by (simp add: AssignI')
+    have "(?w_com, s) \<Rightarrow>\<^bsup> 4 \<^esup> ?inter(''pc'' := ?inter ''pc'' + 1)" using aux1 aux2 by (simp add: Seq)
+    hence aux3: "t = ?inter(''pc'' := ?inter ''pc'' + 1)" using ADD N assms(2) by auto
+
+    have "iexec (x += tmp) (pc, s') = (pc + 1, s'(x :=  s' x + c))" by (simp add: N)
+    hence aux4: "t' = s'(x :=  s' x + c)" using ADD assms(3) by auto
+    
+    show ?thesis using aux3 aux4 by (simp add: assms(5))
+  next
+    case (V y)
+    let ?inter = "s(x := s x + s y)"
+    let ?final = "?inter(''pc'' := ?inter ''pc'' + 1)"
+    let ?w_com = "x ::= (atomExp.V x \<oplus> atomExp.V y) ;; ''pc'' ::= (atomExp.V ''pc'' \<oplus> atomExp.N 1)"
+    have aux1: "(x ::= (atomExp.V x \<oplus> atomExp.V y), s) \<Rightarrow>\<^bsup> 2 \<^esup> ?inter" by (simp add: AssignI')
+    have aux2: "(''pc'' ::= (atomExp.V ''pc'' \<oplus> atomExp.N 1), ?inter) \<Rightarrow>\<^bsup> 2 \<^esup> ?inter(''pc'' := ?inter ''pc'' + 1)" by (simp add: AssignI')
+    have "(?w_com, s) \<Rightarrow>\<^bsup> 4 \<^esup> ?inter(''pc'' := ?inter ''pc'' + 1)" using aux1 aux2 by (simp add: Seq)
+    hence aux3: "t = ?inter(''pc'' := ?inter ''pc'' + 1)" using ADD V assms(2) by auto
+
+    have "iexec (x += tmp) (pc, s') = (pc + 1, s'(x :=  s' x + s' y))" by (simp add: V)
+    hence aux4: "t' = s'(x :=  s' x + s' y)" using ADD assms(3) by auto
+
+    let ?inter' = "s'(x := s' x + s' y)"
+    have "\<forall>z \<noteq> ''pc''. ?inter z = ?inter' z" using ADD V assms(1) assms(5) by auto
+    thus ?thesis using aux3 aux4 by simp
+  qed
+next
+  case (SUB x tmp)
+  then show ?thesis
+  proof (cases tmp)
+    case (N c)
+    let ?inter = "s(x := s x - c)"
+    let ?final = "?inter(''pc'' := ?inter ''pc'' + 1)"
+    let ?w_com = "x ::= (atomExp.V x \<ominus> atomExp.N c) ;; ''pc'' ::= (atomExp.V ''pc'' \<oplus> atomExp.N 1)"
+    have aux1: "(x ::= (atomExp.V x \<ominus> atomExp.N c), s) \<Rightarrow>\<^bsup> 2 \<^esup> ?inter" by (simp add: AssignI')
+    have aux2: "(''pc'' ::= (atomExp.V ''pc'' \<oplus> atomExp.N 1), ?inter) \<Rightarrow>\<^bsup> 2 \<^esup> ?inter(''pc'' := ?inter ''pc'' + 1)" by (simp add: AssignI')
+    have "(?w_com, s) \<Rightarrow>\<^bsup> 4 \<^esup> ?inter(''pc'' := ?inter ''pc'' + 1)" using aux1 aux2 by (simp add: Seq)
+    hence aux3: "t = ?inter(''pc'' := ?inter ''pc'' + 1)" using SUB N assms(2) by auto
+
+    have "iexec (x -= tmp) (pc, s') = (pc + 1, s'(x :=  s' x - c))" by (simp add: N)
+    hence aux4: "t' = s'(x :=  s' x - c)" using SUB assms(3) by auto
+
+    show ?thesis using aux3 aux4 by (simp add: assms(5))
+  next
+    case (V y)
+    let ?inter = "s(x := s x - s y)"
+    let ?final = "?inter(''pc'' := ?inter ''pc'' + 1)"
+    let ?w_com = "x ::= (atomExp.V x \<ominus> atomExp.V y) ;; ''pc'' ::= (atomExp.V ''pc'' \<oplus> atomExp.N 1)"
+    have aux1: "(x ::= (atomExp.V x \<ominus> atomExp.V y), s) \<Rightarrow>\<^bsup> 2 \<^esup> ?inter" by (simp add: AssignI')
+    have aux2: "(''pc'' ::= (atomExp.V ''pc'' \<oplus> atomExp.N 1), ?inter) \<Rightarrow>\<^bsup> 2 \<^esup> ?inter(''pc'' := ?inter ''pc'' + 1)" by (simp add: AssignI')
+    have "(?w_com, s) \<Rightarrow>\<^bsup> 4 \<^esup> ?inter(''pc'' := ?inter ''pc'' + 1)" using aux1 aux2 by (simp add: Seq)
+    hence aux3: "t = ?inter(''pc'' := ?inter ''pc'' + 1)" using SUB V assms(2) by auto
+
+    have "iexec (x -= tmp) (pc, s') = (pc + 1, s'(x :=  s' x - s' y))" by (simp add: V)
+    hence aux4: "t' = s'(x :=  s' x - s' y)" using SUB assms(3) by auto
+    
+    let ?inter' = "s'(x := s' x - s' y)"
+    have "\<forall>z \<noteq> ''pc''. ?inter z = ?inter' z" using SUB V assms(1) assms(5) by auto
+    thus ?thesis using aux3 aux4 by simp
+  qed
+next
+  case (RSH x)
+  let ?inter = "s(x := s x div 2)"
+  let ?final = "?inter(''pc'' := ?inter ''pc'' + 1)"
+  let ?w_com = "x ::= (atomExp.V x \<then>) ;; ''pc'' ::= (atomExp.V ''pc'' \<oplus> atomExp.N 1)"
+  have aux1: "(x ::= (atomExp.V x \<then>), s) \<Rightarrow>\<^bsup> 2 \<^esup> ?inter" by (simp add: AssignI')
+  have aux2: "(''pc'' ::= (atomExp.V ''pc'' \<oplus> atomExp.N 1), ?inter) \<Rightarrow>\<^bsup> 2 \<^esup> ?inter(''pc'' := ?inter ''pc'' + 1)" by (simp add: AssignI')
+  have "(?w_com, s) \<Rightarrow>\<^bsup> 4 \<^esup> ?inter(''pc'' := ?inter ''pc'' + 1)" using aux1 aux2 by (simp add: Seq)
+  hence aux3: "t = ?inter(''pc'' := ?inter ''pc'' + 1)" using RSH assms(2) by auto
+
+  have "iexec (x \<bind>1) (pc, s') = (pc + 1, s'(x :=  s' x div 2))" by simp
+  hence aux4: "t' = s'(x :=  s' x div 2)" using RSH assms(3) by auto
+  
+  show ?thesis using aux3 aux4 by (simp add: assms(5))
+next
+  case (MOD x)
+  let ?inter = "s(x := s x mod 2)"
+  let ?final = "?inter(''pc'' := ?inter ''pc'' + 1)"
+  let ?w_com = "x ::= (atomExp.V x \<doteq>1) ;; ''pc'' ::= (atomExp.V ''pc'' \<oplus> atomExp.N 1)"
+  have aux1: "(x ::= (atomExp.V x \<doteq>1), s) \<Rightarrow>\<^bsup> 2 \<^esup> ?inter" by (simp add: AssignI')
+  have aux2: "(''pc'' ::= (atomExp.V ''pc'' \<oplus> atomExp.N 1), ?inter) \<Rightarrow>\<^bsup> 2 \<^esup> ?inter(''pc'' := ?inter ''pc'' + 1)" by (simp add: AssignI')
+  have "(?w_com, s) \<Rightarrow>\<^bsup> 4 \<^esup> ?inter(''pc'' := ?inter ''pc'' + 1)" using aux1 aux2 by (simp add: Seq)
+  hence aux3: "t = ?inter(''pc'' := ?inter ''pc'' + 1)" using MOD assms(2) by auto
+
+  have "iexec (x %=2) (pc, s') = (pc + 1, s'(x :=  s' x mod 2))" by simp
+  hence aux4: "t' = s'(x :=  s' x mod 2)" using MOD assms(3) by auto
+  
+  show ?thesis using aux3 aux4 by (simp add: assms(5))
+next
+  case (JMP i)
+  have "(''pc'' ::= A (atomExp.N i), s) \<Rightarrow>\<^bsup> 2 \<^esup> s(''pc'' := i)" by (simp add: AssignI')
+  hence aux1: "t = s(''pc'' := i)" using JMP assms(2) by auto
+
+  have "iexec (GOTO i) (pc, s') = (i, s')" by simp
+  hence aux2: "t' = s'" using JMP assms(3) by auto
+
+  show ?thesis using aux1 aux2 by (simp add: assms(5))
+next
+  case (CONDJMP x i)
+  let ?w_com = "IF x\<noteq>0 THEN ''pc'' ::= A (atomExp.N i) ELSE ''pc'' ::= (atomExp.V ''pc'' \<oplus> atomExp.N 1)"
+  consider (c1) "s x = 0" | (c2) "s x > 0" by auto
+  then show ?thesis
+  proof (cases)
+    case c1
+    have "(''pc'' ::= (atomExp.V ''pc'' \<oplus> atomExp.N 1), s) \<Rightarrow>\<^bsup> 2 \<^esup> s(''pc'' := s ''pc'' + 1)" by (simp add: AssignI')
+    hence "(?w_com, s) \<Rightarrow>\<^bsup> 3 \<^esup> s(''pc'' := s ''pc'' + 1)" by (simp add: big_step_t.IfFalse c1)
+    hence aux1: "t = s(''pc'' := s ''pc'' + 1)" using CONDJMP assms(2) by auto
+
+    have "iexec (IF x\<noteq>0 THEN GOTO i) (pc, s') = (pc + 1, s')" using c1 CONDJMP assms(1) assms(5) by auto
+    hence aux2: "t' = s'" using CONDJMP assms(3) by auto
+
+    show ?thesis using aux1 aux2 by (simp add: assms(5))
+  next
+    case c2
+    have "(''pc'' ::= A (atomExp.N i), s) \<Rightarrow>\<^bsup> 2 \<^esup> s(''pc'' := i)" by (simp add: AssignI')
+    hence "(?w_com, s) \<Rightarrow>\<^bsup> 3 \<^esup> s(''pc'' := i)" by (simp add: big_step_t.IfTrue c2)
+    hence aux1: "t = s(''pc'' := i)" using CONDJMP assms(2) fun_upd_eqD by fastforce
+
+    have "iexec (IF x\<noteq>0 THEN GOTO i) (pc, s') = (i, s')" using CONDJMP assms(1) assms(5) c2 by auto
+    hence aux2: "t' = s'" using CONDJMP assms(3) by auto
+
+    show ?thesis using aux1 aux2 by (simp add: assms(5))
+  qed
+qed
+
+theorem single_instr_consist: 
+  assumes "well_defined_instr instr"
+    and "(GOTO_instr_to_WHILE instr, s) \<Rightarrow>\<^bsup> k \<^esup> t"
+    and "iexec instr (pc, s') = (pc', t')" 
+    and "s ''pc'' = pc" and "\<forall>x \<noteq> ''pc''. s x = s' x"
+  shows "t ''pc'' = pc'" and "\<forall>x \<noteq> ''pc''. t x = t' x"
+  using assms(1) assms(2) assms(3) assms(4) assms(5) pc_consist apply auto[1]
+  using assms(1) assms(2) assms(3) assms(4) assms(5) var_consist by presburger
+
+end
